src/Lib/Callback/Dummy.v
@@ -8,23 +8,7 @@ Definition Vprog : varspecs. mk_varspecs prog. Defined.
 
 Open Scope Z.
 
- Definition dummy_callback_spec (z : Z)  : funspec :=
-    WITH data_p : val, size : Z,
-         key_p : val
-    PRE [tarray tuchar z, tuint, tptr tvoid]
-      PROP (0 <= size <= Int.max_unsigned)
-      PARAMS (data_p; Vint (Int.repr size); key_p)
-      GLOBALS ()
-      SEP ()
-    POST [tint]
-      PROP ()
-      LOCAL (temp ret_temp (if size =? 0 then (Vint (Int.repr (-1))) else Vzero))
-      SEP (). 
-
-Definition dummy_callback : ident * funspec :=
-  DECLARE _dummy dummy_callback_spec 32.
-
-(* Definition dummy_callback_spec  : funspec :=
+ Definition dummy_callback_spec : funspec :=
     WITH data_p : val, size : Z,
          key_p : val
     PRE [tptr tvoid, tuint, tptr tvoid]
@@ -34,12 +18,12 @@ Definition dummy_callback : ident * funspec :=
       SEP ()
     POST [tint]
       PROP ()
-      LOCAL (temp ret_temp (if size =? 0 then (Vint (Int.repr (-1))) else Vzero))
+      LOCAL (temp ret_temp (if size <? 0 then (Vint (Int.repr (-1))) else Vzero))
       SEP (). 
 
 Definition dummy_callback : ident * funspec :=
   DECLARE _dummy dummy_callback_spec.
-
+(*
 Definition Gprog := ltac:(with_library prog [dummy_callback]).
 
 Theorem bool_der_encode : semax_body Vprog Gprog f_dummy dummy_callback.
@@ -47,7 +31,7 @@ Proof.
   start_function.
   forward_if (
       PROP ( ) 
-      LOCAL (temp _t'1 (if size =? 0 
+      LOCAL (temp _t'1 (if size <? 0 
                         then (Vint (Int.repr (-1))) 
                         else Vzero);
              temp _buffer data_p; temp _size (Vint (Int.repr size)); 
@@ -61,4 +45,5 @@ Proof.
     entailer!.
     break_if; [rewrite Z.eqb_eq in Heqb; congruence| reflexivity].
   * forward.
-Qed. *)
+Qed. 
+*)
