src/Lib/DWT/ExecDer_write_TL.v
@@ -1,0 +1,61 @@
+Require Import VST.floyd.proofauto.
+Require Import Core.Core Core.Notations Core.Tactics.
+Require Import ExecBer_tlv_tag_serialize
+        ExecBer_tlv_length_serialize.
+
+Open Scope Z.
+
+Definition der_write_TL tag len size := 
+  let (tl, t) := tag_serialize tag (Int.repr size) in
+  let (ll, l) := length_serialize len (Int.repr (size - t)) in
+  let ls := tl ++ ll in
+  if ((t =? -1) || (32 <? t))%bool 
+  then ([], -1)
+  else if l =? -1 
+       then (ls, -1) 
+       else let s := l + t in
+            if 32 <? s 
+            then ([], -1)
+            else (tl ++ ll, s).
+
+Lemma tag_serialize_bounds : forall t l, -1 <= snd (tag_serialize t l) <= 6.
+  { unfold tag_serialize.
+    intros.
+    cbn.
+    repeat break_if; autorewrite with norm; try nia. } 
+Qed.
+
+Lemma length_serialize_bounds : 
+  forall t l, -1 <= snd (length_serialize t l) <= 6.
+  { unfold length_serialize.
+    intros.
+    cbn.
+    repeat break_if; autorewrite with norm; try nia. } 
+Qed.
+
+Lemma der_write_TL_serialize_sum : 
+  forall t l s, 
+    let (tls, tl) := tag_serialize t (Int.repr s)  in
+    let (lls, ll) := length_serialize l (Int.repr (s - tl)) in
+    tl <> -1 ->
+    ll <> -1 ->
+    tl <= 32 ->
+    tl + ll <= 32 ->
+    der_write_TL t l s = (tls ++ lls, tl + ll).
+Proof.
+  intros.
+  repeat break_let.
+  unfold der_write_TL.
+  intros Z Z0 Z32 Zplus.
+  erewrite Heqp.
+  erewrite Heqp0.
+  repeat break_if; try destruct_orb_hyp;
+  repeat Zbool_to_Prop; try nia.
+  intuition.
+Qed.
+
+Definition Z_of_val v := 
+  match v with
+  | Vptr b i => Ptrofs.unsigned i 
+  | _ => 0
+  end.
